{"nbformat":4,"nbformat_minor":0,"metadata":{"colab":{"provenance":[],"authorship_tag":"ABX9TyMWaRveABvuxU5ypkNybPpv"},"kernelspec":{"name":"python3","display_name":"Python 3"},"language_info":{"name":"python"}},"cells":[{"cell_type":"markdown","source":["Consider flow of an incompressible viscous fluid of constant density $\\rho$ and kinematic viscosity $\\nu$, whose velocity $u(x, t)$ and hydrodynamic pressure $p(x, t)$ satisfy the incompressibility condition\n","\\begin{equation}\n","    \\nabla \\cdot u = 0,\n","\\end{equation}\n","and the Navier-Stokes momentum equation\n","\\begin{equation}\n","    \\rho (ut + (u\\cdot\\nabla) u) = -\\nabla p + \\rho\\nu\\nabla^2u.\n","\\end{equation}\n","It follows that the vorticity $\\omega \\equiv \\nabla \\times u$ satisfies\n","\\begin{equation}\n","    \\omega_t + (u\\cdot\\nabla) \\omega - (\\omega\\cdot\\nabla) u = \\nu\\nabla^2\\omega.\n","\\end{equation}\n","If the flow is two-dimensional, then it can be expressed in terms of a streamfunction $\\psi(x, y, t)$, with\n","\\begin{equation}\n","    u â‰¡ (u, v, 0) = \\left( \\frac{\\partial\\psi}{\\partial y} , -\\frac{\\partial\\psi}{\\partial x}, 0 \\right), \\quad \\omega = \\left( 0, 0, -\\nabla^2\\psi\\right),\n","\\end{equation}\n","in terms of which the vorticity equation becomes\n","\\begin{equation}\n","    \\frac{\\partial}{\\partial t}(\\nabla^2\\psi) - \\frac{\\partial (\\psi, \\nabla^2\\psi)}{\\partial (x, y)} = \\nu\\nabla^2(\\nabla^2\\psi).\n","\\end{equation}\n","Suppose there is a stationary rigid boundary on $y = 0$, $x > 0$ on which must be satisfied the conditions of no-slip, $u = 0$, and no penetration, $v = 0$. If the viscosity is 'small', then away from the boundary the flow may, to a good approximation, be irrotational: in this case $u \\approx \\nabla\\phi$ for a\n","velocity potential $\\phi$ satisfying $\\nabla^2\\phi = 0$ (incompressibility) and $\\frac{\\partial\\phi}{\\partial y} = 0$ on $y = 0$, $x > 0$ (no penetration).\n","\n","These conditions, together with corresponding ones on other boundaries and/or\n","at infinity, are sufficient to determine $\\nabla\\phi$ uniquely. As a result, it is not possible to specify the tangential slip velocity component on the boundary, i.e.,\n","\\begin{equation}\n","    \\frac{\\partial\\phi}{\\partial x}(x, 0, t) \\equiv U_e(x, t), \\quad x > 0.\n","\\end{equation}\n","Instead, $U_e(x, t)$ is determined as part of the irrotational potential-flow solution, and is necessarily non-zero. There must therefore be a boundary layer near $y = 0$ where the potential-flow approximation is not valid and satisfaction of the no-slip condition implies viscous diffusion of vorticity away from the boundary.\n","\n","If the boundary layer is 'thin', in the sense that within it $\\frac{\\partial}{\\partial x} \\ll \\frac{\\partial}{\\partial y}$ (i.e., variations with\n","respect to $y$ are much more rapid than variations with respect to $x$), then the approximations\n","\\begin{equation}\n","    \\nabla^2\\psi \\approx \\psi_{yy}, \\quad \\nabla^2(\\nabla2\\psi) \\approx \\psi_{yyyy},\n","\\end{equation}\n","may be made, which can then be integrated once with respect to $y$ to give\n","\\begin{equation}\n","    \\psi_{yt} + \\psi_y\\psi_{xy} - \\psi_x\\psi_{yy} = G(x, t) + \\nu\\psi_{yyy}.\n","\\end{equation}\n","This is in fact the $x$-component of the Navier-Stokes momentum equation with the $\\rho\\nu u_{xx}$ term neglected (since it is small compared to $\\rho\\nu u_{yy}$). The forcing term, or more precisely $-\\rho G$, may be identified with the pressure gradient $\\frac{\\partial p}{\\partial x}$ (which in this approximation is independent of $y$, i.e., uniform across the 'thin' boundary layer). This is to be solved in conjunction with the conditions of no slip and no penetration at the boundary, i.e.,\n","\\begin{equation}\n","    \\psi_y = 0, \\quad -\\psi_x = 0 \\implies \\psi = \\psi_0(t) \\quad \\text{on} \\quad y = 0,\n","\\end{equation}\n","where $\\psi_0(t) = 0$ without loss of generality. In addition the solution must match to the outer potential flow, i.e.,\n","\\begin{equation}\n","    u \\equiv \\psi_y \\implies U_e(x, t) \\quad \\text{as} \\quad y \\to \\infty.\n","\\end{equation}\n","It follows that\n","\\begin{equation}\n","    G(x, t) = \\frac{\\partial U_e}{\\partial t} + U_e\\frac{\\partial U_e}{\\partial x}.\n","\\end{equation}\n","In the special case when the flow is steady, $\\frac{\\partial}{\\partial t} = 0$, and when\n","\\begin{equation}\n","    U_e(x) = Ax^m \\quad \\text{for} \\quad x > 0,\n","\\end{equation}\n","with $A$ and $m$ constants, the problem admits a similarity solution with\n","\\begin{equation}\n","    \\psi(x, y) = |U_e(x)|\\delta(x)f(\\eta), \\quad \\eta = \\frac{y}{\\delta(x)}, \\quad \\delta(x) = \\left(\\frac{\\nu x}{|U_e(x)|}\\right)^{1/2}.\n","\\end{equation}\n","Here, $\\delta(x)$ is a measure of the local boundary-layer thickness, and the function $f$ satisfies the Falkner-Skan equation\n","\\begin{equation}\n","    m(f')^2 - \\frac{1}{2}(m + 1)ff'' = m + f''',\n","\\end{equation}\n","with the boundary conditions\n","\\begin{equation}\n","    f' = f = 0 \\quad \\text{on} \\quad \\eta = 0 \\quad \\text{and} \\quad f' \\to \\mathop{sgn}A \\quad \\text{as} \\quad \\eta \\to \\infty.\n","\\end{equation}\n","In fact, if there is no source of vorticity other than the boundary $y = 0$, then $f'$ should converge to $\\mathop{sgn}A$ exponentially fast as $\\eta \\to \\infty$, i.e.\n","\\begin{equation}\n","    \\eta^N(f' - \\mathop{sgn}A) \\to 0 \\quad \\text{as} \\quad \\eta \\to \\infty,\n","\\end{equation}\n","for all $N$. The tangential velocity component is\n","\\begin{equation}\n","    u = \\frac{\\partial\\psi}{\\partial y} = |U_e(x)|f'(\\eta).\n","\\end{equation}\n","The tangential stress (force per unit area in the $x$-direction) exerted by the fluid on the boundary $y = 0$ is\n","\\begin{equation}\n","    \\tau_0 \\equiv \\rho\\nu\\left.\\frac{\\partial u}{\\partial y}\\right|_{y=0} = \\rho\\left(\\frac{\\nu|U_e(x)|^3}{x}\\right)^{1/2}f''(0).\n","\\end{equation}"],"metadata":{"id":"Lt83ilzG0zpM"}},{"cell_type":"markdown","source":["\n","Different values of $m$ arise for different external flows. Particular cases are (taking $A > 0$ unless stated otherwise):\n","*   $m = 1$: Flow towards a stagnation point on a plane wall.\n","*   $0 < m < 1$: Flow past a wedge of semi-angle $\\theta =\\frac{\\pi m}{m+1}$.\n","*   $m = 0$: Flow past a flat plate (the Blasius boundary layer).\n","*   $-1/2 < m < 0$: Flow around the outside of a corner, turning\n","through an angle $\\theta = -\\frac{\\pi m}{m+1}$ with slip (but no penetration) upstream of the corner, and no slip (and no penetration) downstream.\n","*   $m = -1$: Flow due to a line source (for $A > 0$) or line sink ($A < 0$) at the intersection of two plane rigid boundaries (at arbitrary angle).\n","\n","We ultimately want to solve the two-point-boundary-value problem by shooting,\n","finding by trial-and-error the values of $f''(0)$ which give a solution with the required behaviour as $\\eta \\to \\infty$. Take constants $B \\neq 0$, $k > 0$, $\\eta_0$, $k'$ and $k''$.\n","\n","\n","*   For the case of algebraic convergence, we have the asymptotic behavior:\n","\\begin{align}\n","    f' &= 1 + B\\eta^{-k} + \\cdots \\quad \\text{as} \\quad \\eta \\to \\infty, \\\\\n","    f &= \\eta + C + \\frac{B}{1 - k}\\eta^{1-k} + \\cdots, \\\\\n","    f'' &= -kB\\eta^{-k-1} + \\cdots, \\\\\n","    f''' &= k(k + 1)B\\eta^{-k-2} + \\cdots.\n","\\end{align}\n","By substituting these into the Falkner-Skan equation, we arrive at the following condition\n","\\begin{equation}\n","    k = -\\frac{m}{1 - m}.\n","\\end{equation}\n","Therefore the constant that can be determined without reference to the conditions at $\\eta = 0$ is $k$ and for this behavior to be possible, we must have $m < 1$.\n","\n","*   In the case of exponential convergence, the asymptotic form is given by\n","\\begin{align}\n","    f &= \\eta - \\eta_0 + e^{-\\sigma(\\xi)} + \\cdots \\quad \\text{as} \\quad \\eta \\to \\infty, \\\\\n","    f' &= 1 - \\sigma'e^{-\\sigma} + \\cdots, \\\\\n","    f'' &= (\\sigma')^2e^{-\\sigma} - \\sigma''e^{-\\sigma} + \\cdots, \\\\\n","    f''' &= -(\\sigma')^3e^{-\\sigma} + \\cdots,\n","\\end{align}\n","where $\\xi = \\eta - \\eta_0$ and\n","\\begin{equation}\n","    \\sigma'(\\xi) = k\\xi + k'+ k''\\xi^{-1} + O(\\xi^{-2}).\n","\\end{equation}\n","Substituting these expressions into the Falkner-Skan equation yields\n","\\begin{equation}\n","    -(\\sigma')^3 + \\frac{1}{2}(m + 1)(\\eta_0 - \\xi)(\\sigma')^2 - m = 0.\n","\\end{equation}\n","This leads to the conditions:\n","\\begin{align}\n","    k &= -1, \\\\\n","    k' &= \\frac{1}{2}(m + 1)\\eta_0, \\\\\n","    k'' &= -m - \\frac{1}{4}(m + 1)^2\\eta_0^2. \\\\\n","\\end{align}\n","\n","Thus, the constants $k$, $k'$, and $k''$ can be determined without using the conditions at $\\eta = 0$ and this type of behavior is possible for any value of $m$.\n","\n","*   For algebraic divergence, the solution is given by\n","\\begin{align}\n","    f &= B\\eta^{1+k} + \\cdots \\quad \\text{as} \\quad \\eta \\to \\infty, \\\\\n","    f' &= (1 + k)B\\eta^{k} + \\cdots, \\\\\n","    f'' &= k(1 + k)B\\eta^{k-1} + \\cdots, \\\\\n","    f''' &= (k - 1)k(1 + k)B\\eta^{k-2} + \\cdots.\n","\\end{align}\n","Substituting these into the Falkner-Skan equation gives the leading order equation:\n","\\begin{equation}\n","    (k - 1)k - \\frac{1}{2}(m + 1)k + m = 0.\n","\\end{equation}\n","The solutions are $k = 1$ or $k = m / 2$. Therefore, the constant that can be determined without conditions at $\\eta = 0$ is $k$ and this behavior is possible for any value of $m$.\n","\n","\n","*   In the case of exponential divergence, we have,\n","\\begin{align}\n","    f &= Be^{k\\eta} + \\cdots \\quad \\text{as} \\quad \\eta \\to \\infty, \\\\\n","    f' &= kBe^{k\\eta} + \\cdots, \\\\\n","    f'' &= k^2Be^{k\\eta} + \\cdots, \\\\\n","    f''' &= k^3Be^{k\\eta} + \\cdots.\n","\\end{align}\n","Substituting into the Falkner-Skan equation, we find that at leading order,\n","\\begin{equation}\n","    k^3e^{k\\eta} - \\frac{1}{2}(m + 1)kBe^{\\eta}k^2e^{k\\eta} = 0.\n","\\end{equation}\n","As $\\eta \\to \\infty$, the second term dominates, which means there are no solution of this form. Hence, no constants can be determined and this type of behavior is not possible for any $m$.\n","\n","*   Finally, for a finite-distance singularity, the form is\n","\\begin{align}\n","    f &= B(\\eta_0 - \\eta)^{-1} + \\cdots \\quad \\text{as} \\quad \\eta \\to \\eta_0, \\\\\n","    f' &= B(\\eta_0 - \\eta)^{-2} + \\cdots, \\\\\n","    f'' &= 2B(\\eta_0 - \\eta)^{-3} + \\cdots, \\\\\n","    f''' &= 6B(\\eta_0 - \\eta)^{-4} + \\cdots.\n","\\end{align}\n","Substituting into the Falkner-Skan equation leads to\n","\\begin{equation}\n","    6B - \\frac{1}{2}(m + 1)B^2 = 0.\n","\\end{equation}\n","This gives:\n","\\begin{equation}\n","    B = \\frac{12}{m + 1}.\n","\\end{equation}\n","Thus, the constant $B$ can be determined without the use of conditions at $\\eta$ = 0 and this behavior is possible for any $m  \\neq -1$."],"metadata":{"id":"ulWdGRL17OcH"}}]}