{"nbformat":4,"nbformat_minor":0,"metadata":{"colab":{"provenance":[],"authorship_tag":"ABX9TyNIVwxAwoNSLvPjtRUhI1aJ"},"kernelspec":{"name":"python3","display_name":"Python 3"},"language_info":{"name":"python"}},"cells":[{"cell_type":"markdown","source":["For times $0 \\leq t < \\infty$ we wish to solve the heat equation\n","\n","\\begin{equation}\n","    \\theta_t = \\theta_{xx}\n","\\end{equation}\n","\n","on the interval $0 \\leq x \\leq 1$, with boundary conditions\n","\n","\\begin{equation}\n","    \\theta(0, t) = f(t) \\quad \\text{and} \\quad \\theta(1, t) = 0 \\quad \\text{for} \\quad 0 \\leq t < \\infty, \\quad \\text{where} \\quad f(t) = t(1 âˆ’ t),\n","\\end{equation}\n","\n","and with initial condition\n","\n","\\begin{equation}\n","    \\theta(x, t) = 0 \\quad \\text{for} \\quad t \\leq 0 \\quad \\text{and} \\quad 0 \\leq x \\leq 1.\n","\\end{equation}\n","\n","This is the (non-dimensionalised) initial-value problem for the conduction of heat down a bar when the temperature of one end varies in time. In particular, this can be solved analytically."],"metadata":{"id":"u11V3LsORCcW"}},{"cell_type":"markdown","source":["We first write the ansatz\n","\n","\\begin{equation}\n","    \\theta(x, t) = f(t)(1 - x) + \\phi(x, t).\n","\\end{equation}\n","\n","and compute the relevant derivatives\n","\n","\\begin{align}\n","    \\theta_t &= f'(t)(1 - x) + \\phi_t, \\\\\n","    \\theta_x &= -f(t) + \\phi_x, \\\\\n","    \\theta_{xx} &= \\phi_{xx}. \\\\\n","\\end{align}\n","\n","Then substituting back into the heat equation yields\n","\n","\\begin{equation}\n","    f'(t)(1 - x) + \\phi_t = \\phi_{xx}.\n","\\end{equation}\n","\n","Now consider the boundary conditions for $\\phi(x,t)$. At $x = 0$,\n","\\begin{equation}\n","    f(t) = \\theta(0, t) = f(t)(1 - 0) + \\phi(0, t)  = f(t) + \\phi(0, t),\n","\\end{equation}\n","\n","so $\\phi(0, t) = 0$. At $x = 1$,\n","\n","\\begin{equation}\n","    0 = \\theta(1, t) = f(t)(1 - 1) + \\phi(1, t) = \\phi(1, t),\n","\\end{equation}\n","\n","so $\\phi(1, t) = 0$. Finally, for the the initial condition $\\phi(x,t)$, at $t = 0$,\n","\n","\\begin{equation}\n","    0 = \\theta(x, 0) = f(0)(1 - x) + \\phi(x, 0) = \\phi(x, 0),\n","\\end{equation}\n","\n","so $\\phi(x, 0) = 0$. To solve for $\\phi$ using a Fourier sine series, we assume a solution of the form\n","\n","\\begin{equation}\n","    \\phi(x, t) = \\sum_{n=1}^{\\infty} B_n(t) \\sin(n\\pi x).\n","\\end{equation}\n","\n","Let $G(x, t) = -f'(t)(1 - x)$. The coefficients for the Fourier sine series of $G(x, t)$ are given by:\n","\n","\\begin{align}\n","    G_n(t) &= \\frac{2}{1} \\int_{0}^{1} G(x, t) \\sin(n\\pi x) \\,dx \\\\\n","    &= 2 \\int_{0}^{1} -f'(t)(1 - x) \\sin(n\\pi x) \\,dx\n","\\end{align}\n","\n","Using integration by parts,\n","\n","\\begin{align}\n","    \\int_{0}^{1} (1 - x) \\sin(n\\pi x) \\,dx &= \\left[ -\\frac{1 - x}{n\\pi} \\cos(n\\pi x) \\right]_{0}^{1} - \\int_{0}^{1} \\frac{1}{n\\pi} \\cos(n\\pi x) \\,dx \\\\\n","    &= \\left[ (0) - \\left( -\\frac{1}{n\\pi} \\cos(0) \\right) \\right] - \\left[ \\frac{1}{(n\\pi)^2} \\sin(n\\pi x) \\right]_{0}^{1} \\\\\n","    &= \\frac{1}{n\\pi} - \\left[ \\frac{1}{(n\\pi)^2} (0 - 0) \\right] = \\frac{1}{n\\pi}\n","\\end{align}\n","\n","So, $G_n(t) = -\\frac{2f'(t)}{n\\pi}$.\n","\n","Now, substitute the Fourier series $\\phi(x, t) = \\sum_{n=1}^{\\infty} B_n(t) \\sin(n\\pi x)$ into the governing equation for $\\phi$,\n","\n","\\begin{equation}\n","    \\sum_{n=1}^{\\infty} B_n'(t) \\sin(n\\pi x) = \\sum_{n=1}^{\\infty} B_n(t) (-n^2\\pi^2) \\sin(n\\pi x) + \\sum_{n=1}^{\\infty} G_n(t) \\sin(n\\pi x).\n","\\end{equation}\n","\n","Equating coefficients for each $\\sin(n\\pi x)$ gives\n","\n","\\begin{equation}\n","    B_n'(t) + n^2\\pi^2 B_n(t) = G_n(t) = -\\frac{2f'(t)}{n\\pi}.\n","\\end{equation}\n","\n","This is a first-order linear ODE. We can solve it using an integrating factor,\n","\n","\\begin{equation}\n","    \\exp\\left(\\int n^2\\pi^2 \\,dt\\right) = \\exp(n^2\\pi^2 t),\n","\\end{equation}\n","\n","where\n","\n","\\begin{equation}\n","    \\frac{d}{dt} (B_n(t) e^{n^2\\pi^2 t}) = -\\frac{2f'(t)}{n\\pi} e^{n^2\\pi^2 t}.\n","\\end{equation}\n","\n","Integrate both sides with respect to $t$,\n","\n","\\begin{equation}\n","    B_n(t) e^{n^2\\pi^2 t} = \\int_{0}^{t} -\\frac{2f'(\\tau)}{n\\pi} e^{n^2\\pi^2 \\tau} \\,d\\tau + C_n\n","\\end{equation}\n","\n","From the initial condition $\\phi(x, 0) = 0$, we obtain $B_n(0) = 0$. So, $C_n = 0$. Thus,\n","\n","\\begin{equation}\n","    B_n(t) = -\\frac{2}{n\\pi} e^{-n^2\\pi^2 t} \\int_{0}^{t} f'(\\tau) e^{n^2\\pi^2 \\tau} \\,d\\tau.\n","\\end{equation}\n","\n","Recall that $f(t) = t(1-t) = t - t^2$, so $f'(t) = 1 - 2t$. Finally,\n","\n","\\begin{equation}\n","    B_n(t) = -\\frac{2}{n\\pi} e^{-n^2\\pi^2 t} \\int_{0}^{t} (1 - 2\\tau) e^{n^2\\pi^2 \\tau} d\\tau.\n","\\end{equation}\n","\n","This integral can be solved using integration by parts, eventually yielding\n","\\begin{equation}\n","    B_n(t) = \\frac{2}{(n\\pi)^5}\\left[2t(n\\pi)^2 + ((n\\pi)^2 + 2)(e^{-(n\\pi)^2 t} - 1)\\right].\n","\\end{equation}"],"metadata":{"id":"O_wVNXFvVoB9"}},{"cell_type":"markdown","source":["As $t \\to \\infty$, the exponential terms $e^{-n^2\\pi^2 t}$ will cause $B_n(t)$ to decay unless the integral term grows with $t$. This suggests looking at the steady-state behavior or dominant terms for large $t$.\n","\n","Let's consider the general form of\n","\n","\\begin{equation}\n","    B_n(t) = -\\frac{2}{n\\pi} e^{-n^2\\pi^2 t} \\int_{0}^{t} f'(\\tau) e^{n^2\\pi^2 \\tau} \\,d\\tau.\n","\\end{equation}\n","\n","We can use integration by parts for the integral\n","\n","\\begin{align}\n","    \\int_{0}^{t} f'(\\tau) e^{n^2\\pi^2 \\tau} d\\tau &= \\left[ f'(\\tau) \\frac{e^{n^2\\pi^2 \\tau}}{n^2\\pi^2} \\right]_{0}^{t} - \\int_{0}^{t} f''(\\tau) \\frac{e^{n^2\\pi^2 \\tau}}{n^2\\pi^2} \\,d\\tau \\\\\n","    &= \\frac{f'(t) e^{n^2\\pi^2 t}}{n^2\\pi^2} - \\frac{f'(0)}{n^2\\pi^2} - \\frac{1}{n^2\\pi^2} \\int_{0}^{t} f''(\\tau) e^{n^2\\pi^2 \\tau} d\\tau.\n","\\end{align}\n","\n","\n","Substitute this back into $B_n(t)$\n","\n","\\begin{align}\n","    B_n(t) &= -\\frac{2}{n\\pi} e^{-n^2\\pi^2 t} \\left( \\frac{f'(t) e^{n^2\\pi^2 t}}{n^2\\pi^2} - \\frac{f'(0)}{n^2\\pi^2} - \\frac{1}{n^2\\pi^2} \\int_{0}^{t} f''(\\tau) e^{n^2\\pi^2 \\tau} \\,d\\tau \\right) \\\\\n","    &= -\\frac{2f'(t)}{n^3\\pi^3} + \\frac{2f'(0)}{n^3\\pi^3} e^{-n^2\\pi^2 t} + \\frac{2}{n^3\\pi^3} e^{-n^2\\pi^2 t} \\int_{0}^{t} f''(\\tau) e^{n^2\\pi^2 \\tau} d \\,\\tau.\n","\\end{align}\n","\n","We have $f'(t) = 1-2t$ so $f''(t) = -2$, hence\n","\n","\\begin{align}\n","    B_n(t) &= -\\frac{2(1-2t)}{n^3\\pi^3} + \\frac{2}{n^3\\pi^3} e^{-n^2\\pi^2 t} + \\frac{2}{n^3\\pi^3} e^{-n^2\\pi^2 t} \\int_{0}^{t} (-2) e^{n^2\\pi^2 \\tau} \\,d\\tau \\\\\n","    &= -\\frac{2(1-2t)}{n^3\\pi^3} + \\frac{2}{n^3\\pi^3} e^{-n^2\\pi^2 t} - \\frac{4}{n^3\\pi^3} e^{-n^2\\pi^2 t} \\left[ \\frac{e^{n^2\\pi^2 \\tau}}{n^2\\pi^2} \\right]_{0}^{t} \\\\\n","    &= -\\frac{2(1-2t)}{n^3\\pi^3} + \\frac{2}{n^3\\pi^3} e^{-n^2\\pi^2 t} - \\frac{4}{n^5\\pi^5} e^{-n^2\\pi^2 t} (e^{n^2\\pi^2 t} - 1)\n","\\end{align}\n","\n","As $ t\\to \\infty$, the terms with $e^{-n^2\\pi^2 t}$ go to zero. So, for large $t$,\n","\n","\\begin{equation}\n","    B_n(t) \\approx \\frac{4t}{n^3\\pi^3} - \\frac{2}{n^3\\pi^3} - \\frac{4}{n^5\\pi^5}.\n","\\end{equation}\n","\n","Now, substitute this back into $\\phi(x, t) = \\sum_{n=1}^{\\infty} B_n(t) \\sin(n\\pi x)$\n","\n","\\begin{equation}\n","    \\phi(x, t) \\approx \\left( \\sum_{n=1}^{\\infty} \\frac{4}{n^3\\pi^3} \\sin(n\\pi x) \\right) t + \\left( \\sum_{n=1}^{\\infty} \\left( -\\frac{2}{n^3\\pi^3} - \\frac{4}{n^5\\pi^5} \\right) \\sin(n\\pi x) \\right).\n","\\end{equation}\n","\n","This is the limiting steady state solution for the initial value problem."],"metadata":{"id":"tpNEKv4K4iIa"}},{"cell_type":"code","source":["import numpy as np\n","\n","def f(t):\n","    '''\n","    Function f(t) = t(1-t).\n","    '''\n","    return t * (1 - t)\n","\n","def alpha(x, num_terms=100):\n","    '''\n","    Computes alpha(x) from the Fourier series.\n","    '''\n","    pi = np.pi\n","    alpha_sum = sum(\n","        (4 / (n**3 * pi**3)) * np.sin(n*pi*x)\n","        for n in range(1, num_terms + 1)\n","        )\n","    return alpha_sum\n","\n","def beta(x, num_terms=100):\n","    '''\n","    Computes beta(x) from the Fourier series.\n","    '''\n","    pi = np.pi\n","    beta_sum = sum(\n","        (-2 / (n**3 * pi**3) - 4 / (n**5 * pi**5)) * np.sin(n*pi*x)\n","        for n in range(1, num_terms + 1)\n","        )\n","    return beta_sum\n","\n","def theta_asymptotic(x, t):\n","    '''\n","    Computes the asymptotic analytic solution for large t.\n","    '''\n","    return f(t) * (1 - x) + alpha(x) * t + beta(x)"],"metadata":{"id":"Qp9YIVASFyk7","executionInfo":{"status":"ok","timestamp":1757448630451,"user_tz":-60,"elapsed":9,"user":{"displayName":"Alex Zhou","userId":"15814347624889041767"}}},"execution_count":1,"outputs":[]}]}