{"nbformat":4,"nbformat_minor":0,"metadata":{"colab":{"provenance":[],"authorship_tag":"ABX9TyObXpDvuy68OcoKFNJTSzuV"},"kernelspec":{"name":"python3","display_name":"Python 3"},"language_info":{"name":"python"}},"cells":[{"cell_type":"markdown","source":["The Korteweg-de Vries (KdV) equation is given by\n","\\begin{equation}\n","    u_t + uu_x + \\delta^2u_{xxx} = 0.\n","\\end{equation}\n","It arises in many branches of physics as a model for the evolution and interaction of nonlinear waves. It is well-known that the equation possesses single-soliton solutions of the form $u(x, t) = f(x − ct)$ where\n","\\begin{equation}\n","    f(x) = \\frac{A}{\\cosh^2 \\left(x − x_0/\\Delta\\right)}, \\quad \\Delta^2 = 12\\delta^2/A, \\quad c = A/3,\n","\\end{equation}\n","and where $A$ and $x_0$ are arbitrary constants representing the amplitude and initial location of the soliton respectively. It is supposed that u(x, t) obeys the cyclic boundary conditions,\n","\\begin{equation}\n","    u(x + 1, t) = u(x, t),\n","\\end{equation}\n","so that only the region $0 \\leq x \\leq 1$ need be considered.\n","\n","To verify the solution, we must compute the partial derivatives of $u(x,t)$ and substitute them into the KdV equation. Let $z = (x - x0 - ct) / \\Delta$. We have\n","\\begin{align}\n","    u_t &= (2Ac / \\Delta) \\tanh(z) / \\cosh^2(z) \\\\\n","    u_x &= (-2A / \\Delta) \\tanh(z)  / \\cosh^2(z) \\\\\n","    u_{xxx} &= (-8A / \\Delta^3) \\tanh(z) / \\cosh^2(z) + (24A / \\Delta^3) \\tanh(z) / \\cosh^4(z)\n","\\end{align}\n","Set $T = \\tanh(z)/\\cosh^2(z)$ and $S = \\tanh(z)/\\cosh^2(z)$. Now, substituting these derivatives into the KdV equation yields\n","\\begin{equation}\n","    (2Ac / \\Delta)T + (-2^2A / \\Delta)S  + \\delta^2 [(-8A / \\Delta^3)T + (24A / \\Delta^3)S] = 0,\n","\\end{equation}\n","and grouping by $T$ and $S$ gives\n","\\begin{equation}\n","[ (2Ac / \\Delta) - (8A\\delta^2 / \\Delta^3) ] T + [ (-2A^2 / \\Delta) + (24A\\delta^2 / \\Delta^3) ] S = 0.\n","\\end{equation}\n","For this equation to hold true for all values of $z$, the coefficients of both terms must be zero. From the T term,\n","\\begin{equation}\n","    2Ac / \\Delta = 8A\\delta^2 / \\Delta^3 \\implies c = 4δ^2 / Δ^2.\n","\\end{equation}\n","From the sech^4(z)tanh(z) term,\n","\\begin{equation}\n","    2A^2 / \\Delta = 24A\\delta^2 / \\Delta^3 \\implies A = 12\\delta^2 / \\Delta^2.\n","\\end{equation}\n","This is consistent with the conditions given for the coefficients."],"metadata":{"id":"7qrfiXTNCD38"}},{"cell_type":"markdown","source":["\n","---\n","\n","The KdV equation is known to have an infinite number of conserved quantities for solutions that decay at infinity or are periodic.\n","\n","The mass is defined as\n","\\begin{equation}\n","    M = \\int_0^1 u(x, t) \\,dx\n","\\end{equation}\n","To show it is independent of time, we must show that its time derivative is zero. We have\n","\\begin{align}\n","    \\frac{dM}{dt}\n","    &= \\int_0^1 \\frac{\\partial u}{\\partial t} \\,dx = \\int_0^1 u_t \\,dx \\\\\n","    &= \\int_0^1 (-uu_x - \\delta^2 u_{xxx}) \\,dx \\\\\n","    &= -\\int_0^1 uu_x \\,dx - \\delta^2 \\int_0^1 u_{xxx} \\,dx\n","\\end{align}\n","We evaluate each integral. The first integral is\n","\\begin{equation}\n","    \\int_0^1 uu_x \\,dx = \\int_0^1 \\frac{1}{2} \\frac{d}{dx}(u^2) \\,dx = \\left[\\frac{1}{2}u^2\\right]_0^1 = \\frac{1}{2}[u(1,t)^2 - u(0,t)^2].\n","\\end{equation}\n","Due to the periodic boundary condition $u(1,t) = u(0,t)$, this term is zero. The second integral is\n","\\begin{equation}\n","    \\int_0^1 u_{xxx} \\,dx = [u_{xx}]_0^1 = u_{xx}(1,t) - u_{xx}(0,t).\n","\\end{equation}\n","Since $u$ is periodic, its derivatives are also periodic, so this term is also zero. Therefore, the mass $M$ is conserved over time.\n","\n","The energy is defined as\n","\\begin{equation}\n","    E = \\int_0^1 \\frac{1}{2} u^2(x, t) \\,dx.\n","\\end{equation}\n","Once again, we shall show that its time derivative is zero (dE/dt = 0). We have\n","\\begin{align}\n","    \\frac{dE}{dt}\n","    &= \\int_0^1 \\frac{1}{2} 2u \\frac{\\partial u}{\\partial t} \\,dx = \\int_0^1 uu_t \\,dx \\\\\n","    &= \\int_0^1 u(-uu_x - \\delta^2 u_{xxx}) \\,dx \\\\\n","    &= -\\int_0^1 u^2 u_x \\,dx - \\delta^2 \\int_0^1 uu_{xxx} \\,dx\n","\\end{align}\n","The first integral is evaluated as\n","\\begin{equation}\n","    -\\int_0^1 u^2u_x \\,dx = -\\int_0^1 \\frac{1}{3} \\frac{d}{dx}(u^3) \\,dx = \\left[-\\frac{1}{3}u^3\\right]_0^1 = -\\frac{1}{3}[u(1,t)^3 - u(0,t)^3].\n","\\end{equation}\n","Due to periodicity, this term is zero.\n","For the second integral, we use parts,\n","\\begin{equation}\n","    - \\delta^2 \\int_0^1 uu_{xxx} \\,dx = -\\delta^2 \\left([uu_{xx}]_0^1 - \\int_0^1 u_xu_{xx} \\,dx \\right)\n","\\end{equation}\n","The boundary term is zero due to periodicity. The integral becomes\n","\\begin{equation}\n","    \\delta^2\\int_0^1 u_xu_{xx} \\,dx = \\delta^2\\int_0^1 \\frac{1}{2} \\frac{d}{dx}(ux)^2 \\,dx = δ^2\\left[\\frac{1}{2}(ux)^2\\right]_0^1.\n","\\end{equation}\n","This term is also zero due to the periodicity of $u_x$. Therefore, the energy $E$ is also conserved over time."],"metadata":{"id":"H6A3B4IRMH19"}}]}