{"nbformat":4,"nbformat_minor":0,"metadata":{"colab":{"provenance":[],"authorship_tag":"ABX9TyOzTjAT99JRydPsRlEr3iGL"},"kernelspec":{"name":"python3","display_name":"Python 3"},"language_info":{"name":"python"}},"cells":[{"cell_type":"markdown","source":["The angular velocity with respect to principal axes of inertia in a rigid body is taken to be\n","\\begin{equation}\n","    \\omega = (\\omega_1, \\omega_2, \\omega_3).\n","\\end{equation}\n","If the principal moments of inertia are $A$, $B$, $C$ with respect to these axes, then the angular momentum is\n","\\begin{equation}\n","    h = (A\\omega_1, B\\omega_2, C\\omega_3).\n","\\end{equation}\n","These axes are fixed in the body and have angular velocity $\\omega$ with respect to an inertial frame instantaneously coincident with the principal axes. The rate of change of angular momentum with respect to such an inertial frame is\n","\\begin{equation}\n","    \\frac{dh}{dt} + \\omega \\wedge h.\n","\\end{equation}\n","In the case when there is no net moment of external forces acting on the body, the law 'rate of change of angular momentum = moment of external forces' gives\n","\\begin{equation}\n","    \\frac{dh}{dt} + \\omega \\wedge h = 0.\n","\\end{equation}\n","Expanding this equation into components gives\n","\\begin{equation}\n","    \\begin{cases}\n","        A\\frac{d\\omega_1}{dt} + (C - B)\\omega_2\\omega_3 = 0 \\\\\n","        B\\frac{d\\omega_2}{dt} + (A - C)\\omega_3\\omega_1 = 0 \\\\\n","        C\\frac{d\\omega_3}{dt} + (B - A)\\omega_1\\omega_2 = 0\n","    \\end{cases}\n","\\end{equation}\n","It can be shown analytically that these equations have two first integrals, which say that the energy and the magnitude of the angular momentum remain constant, as follows\n","\\begin{equation}\n","    \\frac{1}{2}A\\omega_1^2 + \\frac{1}{2}B\\omega_2^2 + \\frac{1}{2}C\\omega_3^2 = E, \\\\\n","    A^2\\omega_1^2 + B^2\\omega_2^2 + C^2\\omega_3^2 = H^2.\n","\\end{equation}\n","Since the moment of external forces is zero, we also know that the angular momentum vector $h$ is constant when measured in an inertial frame.\n"],"metadata":{"id":"94fWvkSSy2C_"}},{"cell_type":"code","source":["import numpy as np\n","from scipy.integrate import solve_ivp\n","import matplotlib.pyplot as plt\n","\n","def euler_equations(t, w, params):\n","    '''\n","    Defines the system of differential equations for a rigid body.\n","    '''\n","    A, B, C = params\n","    w1, w2, w3 = w\n","    dw1dt = (B - C) / A * w2 * w3\n","    dw2dt = (C - A) / B * w3 * w1\n","    dw3dt = (A - B) / C * w1 * w2\n","    return [dw1dt, dw2dt, dw3dt]\n","\n","def calculate_conserved_quantities(w, params):\n","    '''\n","    Calculates and returns the energy and squared angular momentum.\n","    '''\n","    A, B, C = params\n","    w1, w2, w3 = w\n","    energy = 0.5 * (A * w1**2 + B * w2**2 + C * w3**2)\n","    angular_momentum_sq = (A * w1)**2 + (B * w2)**2 + (C * w3)**2\n","    return energy, angular_momentum_sq\n","\n","def solve_equations(params, w_initial, t_span, t_eval):\n","    '''\n","    Solves the ODE system and returns the solution object.\n","    '''\n","    return solve_ivp(\n","        euler_equations,\n","        t_span,\n","        w_initial,\n","        args=(params,),\n","        dense_output=True,\n","        t_eval=t_eval,\n","        rtol=1e-8,\n","        atol=1e-8\n","    )\n","\n"],"metadata":{"id":"YmNLoTLOoYwm","executionInfo":{"status":"ok","timestamp":1761702661802,"user_tz":0,"elapsed":53,"user":{"displayName":"Alex Zhou","userId":"15814347624889041767"}}},"execution_count":7,"outputs":[]},{"cell_type":"code","source":["def plot_time_series(t, w_components):\n","    '''\n","    Generates and displays the time series plot.\n","    '''\n","    w1, w2, w3 = w_components\n","    plt.figure(figsize=(8, 5))\n","    plt.plot(t, w1, label=f'ω_1(t)')\n","    plt.plot(t, w2, label=f'ω_2(t)')\n","    plt.plot(t, w3, label=f'ω_3(t)')\n","    plt.title(\"Angular Velocity Components vs. Time\")\n","    plt.xlabel(f\"Time $(t)$\")\n","    plt.ylabel(\"Angular Velocity (rad/s)\")\n","    plt.legend()\n","    plt.grid(True)\n","    plt.show()\n","\n","def plot_phase_space(w_components):\n","    '''\n","    Generates and displays the 3D phase space plot.\n","    '''\n","    w1, w2, w3 = w_components\n","    fig = plt.figure(figsize=(8, 6))\n","    ax = fig.add_subplot(111, projection='3d')\n","    ax.plot(w1, w2, w3)\n","    ax.scatter(w1[0], w2[0], w3[0], color='red', s=50, label='Start Point')\n","    ax.set_title(\"3-D Phase Space Plot of Angular Velocity\")\n","    ax.set_xlabel(f\"$ω_1$ (OX axis)\")\n","    ax.set_ylabel(f\"$ω_2$ (OY axis)\")\n","    ax.set_zlabel(f\"$ω_3$ (OZ axis)\")\n","    ax.legend()\n","    plt.show()"],"metadata":{"id":"tpfYA6_io7Pn","executionInfo":{"status":"ok","timestamp":1761702661804,"user_tz":0,"elapsed":6,"user":{"displayName":"Alex Zhou","userId":"15814347624889041767"}}},"execution_count":8,"outputs":[]},{"cell_type":"markdown","source":["Since $A$, $B$, $C$, $\\omega_1(0)$, $\\omega_2(0)$ and $\\omega_3(0)$ may all in principle take arbitrary values, the parameter space to be explored appears at first to be quite large. If $A$, $B$ and $C$ take distinct values, then in our results, we can take $A > B > C$ as any other ordering simply corresponds to a relabeling of the principal axes. We are cyclicly permuting the Euler equations.\n","\n","The dynamics simplify significantly if any of the principal moments of inertia are equal. In the case of a symmetric top, we have two equal moments. Assume that $A = B$. Then the third Euler equation becomes\n","\\begin{equation}\n","    C\\frac{d\\omega_3}{dt} + (B - A)\\omega_1\\omega_2 = 0.\n","\\end{equation}\n","This implies that $\\frac{d\\omega_3}{dt} = 0$, so the angular velocity component along the unique axis $\\omega_3$ is constant. The angular velocity vector $\\omega$ is not constant but precesses around this axis of symmetry at a constant rate. Finally, in the case of a spherical top, all three moments are equal $A = B = C$. Now, all the difference terms in Euler's equations become zero, so all components of $\\omega$ are constant. Therefore, the angular velocity vector $\\omega$ is constant in the body frame. Since there is no external torque, the angular momentum vector $h = I\\omega = A\\omega$ is constant in the inertial frame. The body rotates with a completely constant angular velocity, exhibiting no precession or tumbling.\n","\n","We can set $B = 1$ without loss of generality. This simplification comes from the fact that the dynamics described by Euler's equations depend only on the ratios of the moments of inertia, not their absolute values. We can show this by dividing Euler's equations by $B$, which shows that the behavior of the system is now governed by the two ratios $A/B$ and $C/B$.\n","\n","Choosing the rotational kinetic energy $E = 1$ is equivalent to choosing a new unit of time. Start with a solution $\\omega(t)$ to Euler's equations that has energy\n","\\begin{equation}\n","    E = \\frac{1}{2}(A\\omega_1^2 + B\\omega_2^2 + C\\omega_3^2).\n","\\end{equation}\n","Introduce a scaled time variable $\\tau = \\lambda t$ and a new angular velocity vector $\\Omega(\\tau) = c\\omega(t)$, where $\\lambda$ is a constant scaling factor for time and $c$ is a constant scaling factor for velocity. Using the chain rule, the derivative with respect to the new time is\n","\\begin{equation}\n","    \\frac{d}{d\\tau} = \\frac{dt}{d\\tau}\\frac{d}{dt} = \\frac{1}{\\lambda}\\frac{d}{dt}.\n","\\end{equation}\n","Now, substitute $\\omega = \\Omega/c$ and the new derivative into the first Euler equation to obtain\n","\\begin{equation}\n","    A\\lambda \\frac{d(\\Omega_1/c)}{dτ} + (C - B)\\frac{\\Omega_2}{c}\\frac{\\Omega_3}{c} = \\frac{A\\lambda}{c}\\frac{d\\Omega_1}{d\\tau} + \\frac{C - B}{c^2}\\Omega_2\\Omega_3 = 0. \\\\\n","    \\implies A\\frac{d\\Omega_1}{d\\tau} + \\frac{C - B}{c\\lambda}\\Omega_2\\Omega_3 = 0.\n","\\end{equation}\n","For this to match the standard Euler form, we require $c\\lambda = 1$ or $\\lambda = 1/c$. The energy of the new solution is\n","\\begin{equation}\n","    E' = \\frac{1}{2}(A\\Omega_1^2 + B\\Omega_2^2 + C\\Omega_3^2) = \\frac{1}{2}c^2(A\\omega_1^2 + B\\omega_2^2 + C\\omega_3^2)\n","\\end{equation}\n","or $E' = c^2E$.\n","We want to choose our scaling factor such that $E' = 1$. This means that $c = 1/\\sqrt{E}$ and $\\lambda = \\sqrt{E}$. This is equivalent to re-scaling the time variable to $\\tau = t/\\sqrt{E}$."],"metadata":{"id":"9-hR25XeqZpV"}}]}