{"nbformat":4,"nbformat_minor":0,"metadata":{"colab":{"provenance":[],"authorship_tag":"ABX9TyMfFOA5KcQAmPe8KL11EVVV"},"kernelspec":{"name":"python3","display_name":"Python 3"},"language_info":{"name":"python"}},"cells":[{"cell_type":"markdown","source":["We shall investigate the motion of a particle or photon in the Schwarzschild solution to the Einstein field equations.\n","\n","Use the Lagrangian for a partial in the equatorial place of a Schwarzschild metric\n","\\begin{equation}\n","    L = F(r)\\dot{t}^2 - \\frac{\\dot{r}^2}{F(r)} - (r\\dot\\phi)^2,\n","\\end{equation}\n","where $F(r) = 1 - 1/r$, and we differentiate with respect to a variable $s$ which is an affine parameter along the geodesic. We choose dimensionless units such that $c = 1$ and $2GM = 1$ which makes the Schwarzschild radius $r = 1$. Lagrange's equation for a coordinate $q_i$ is given by\n","\\begin{equation}\n","    \\frac{d}{ds} \\frac{\\partial L}{\\partial \\dot{q}_i} - \\frac{\\partial L}{\\partial q_i} = 0.\n","\\end{equation}\n","We apply Lagrange's equation to the coordinates $t$ and $\\phi$. For the t-coordinate, since the Lagrangian does not explicitly depend on $t$, that is $\\frac{\\partial L}{\\partial t} = 0$, the coordinate is cyclic and it implies a conserved quantity,\n","\\begin{equation}\n","    \\frac{\\partial L}{\\partial \\dot{t}} = 2F(r)\\dot{t}.\n","\\end{equation}\n","Lagrange's equation becomes\n","\\begin{equation}\n","    \\frac{d}{ds} (2F(r)\\dot{t}) = 0\n","\\end{equation}\n","This means that $E = F(r)\\dot{t}$ is a constant which represents the conserved energy per unit mass. For the \\phi -coordinate, similarly, the Lagrangian does not explicitly depend on $\\phi$, or $\\frac{\\partial L}{\\partial \\phi} = 0$. Hence\n","\\begin{equation}\n","    \\frac{\\partial L}{\\partial \\dot\\phi} = -2r^2\\dot\\phi,\n","\\end{equation}\n","so Lagrange's equation becomes\n","\\begin{equation}\n","    \\frac{d}{ds} (-2r^2\\dot\\phi) = 0.\n","\\end{equation}\n","This implies that $h = r^2\\dot\\phi$ is also a constant which represents the conserved angular momentum per unit mass.\n","\n","Instead of using Lagrange's equation for the $r$ coordinate, we can use the Lagrangian itself as a third equation of motion. The value of the Lagrangian $L$ is constant along a geodesic. For massive particles, the affine parameter $s$ can be chosen as the proper time $\\tau$, which normalises the Lagrangian to $L = 1$. For photons which travel along null geodesics, we have $L = 0$. The equation is\n","\\begin{equation}\n","    L = (1 - 1/r)\\dot{t}^2 - \\frac{\\dot{r}^2}{1 - 1/r} - r^2\\dot\\phi^2.\n","\\end{equation}\n","Now, we substitute the conserved quantities $E$ and $h$,\n","\\begin{equation}\n","    L = \\frac{E^2}{1 - 1/r} - \\frac{\\dot{r}^2}{1 - 1/r} - \\frac{h^2}{r^2}.\n","\\end{equation}\n","To get the equation for the orbit shape, we change the variable from $r$ to $u = 1/r$ and the independent variable from $s$ to $\\phi$. By the chain rule,\n","\\begin{equation}\n","    \\dot{r} = \\frac{dr}{ds} = \\frac{dr}{du}\\frac{du}{d\\phi}\\frac{d\\phi}{ds} = \\frac{-1}{u^2}\\frac{du}{d\\phi}(hu^2) = -h\\frac{du}{d\\phi}.\n","\\end{equation}\n","Substituting $u$ and $\\dot{r}$ into the equation for $L$ yields\n","\\begin{equation}\n","    L = \\frac{E^2 - h^2(\\frac{du}{d\\phi})^2}{1 - u} - h^2u^2,\n","\\end{equation}\n","which rearranges to\n","\\begin{equation}\n","    h^2\\left(\\frac{du}{d\\phi}\\right)^2 = E^2 - (1 - u)(L + h^2u^2).\n","\\end{equation}\n","\n","To find the orbit equation involving the second derivative, we differentiate the above expression with respect to $\\phi$, using the chain rule $\\frac{d}{d\\phi} = \\frac{du}{d\\phi}\\frac{d}{du}$,\n","\\begin{align}\n","    2h^2\\frac{du}{d\\phi}\\frac{d^2u}{d\\phi^2}\n","    &= -\\frac{d}{d\\phi}((1 - u)(L + h^2u^2)) \\\\\n","    &= -\\frac{du}{d\\phi}\\frac{d}{du}(L + h^2u^2 - Lu - h^2u^3) \\\\\n","    &= -\\frac{du}{d\\phi}(2h^2u - L - 3h^2u^2)\n","\\end{align}\n","Cancelling out the derivative and rearranging gives the general orbit equation,\n","\\begin{equation}\n","    \\frac{d^2u}{d\\phi^2} + u = \\frac{L}{2h^2} + \\frac{3u^2}{2}.\n","\\end{equation}\n","For massive particles, setting $L = 1$, and recalling that $2GM = 1$, we get\n","\\begin{equation}\n","    \\frac{d^2u}{d\\phi^2} + u = \\frac{1}{2h^2} + \\frac{3u^2}{2}.\n","\\end{equation}\n","This equation describes the orbits of planets or stars around a non-rotating black hole. The final term is a relativistic correction that accounts for the precession of perihelia.\n","For massless particles, setting $L = 0$, the equation simplifies to\n","\\begin{equation}\n","    \\frac{d^2u}{d\\phi^2} + u = \\frac{3u^2}{2}.\n","\\end{equation}\n","This equation governs the path of light in the Schwarzschild spacetime, which predicts the gravitational lensing of light by massive objects.\n"],"metadata":{"id":"iovsZeQtSdjZ"}}]}